src/semantics.lean
@@ -1,0 +1,32 @@
+-- (C) Copyright 2019, Hans-Dieter Hiep
+
+import syntax
+
+universes u
+variables (α : Type) (β : Type)
+
+open type
+
+/-
+We treat objects transparently.
+Each object is associated to a single class name.
+Given a set of objects, we can always construct some new object.
+-/
+class objects [global_names α] :=
+(class_of: β → class_name α)
+(new: finset β → β)
+(new_is_new: ∀x : finset β, (new x) ∉ x)
+
+def objects.type_of [global_names α] [objects α β] (o : β) : type α :=
+    ref (objects.class_of α o)
+
+open objects
+
+/-
+We treat values as being of a type.
+A value of a reference type is an object of the same class.
+A value of a data type is a term of the type in the host language.
+-/
+inductive value [global_names α] [objects α β] : type α → Type 1
+| obj (o : β) : value (type_of α β o)
+| term {γ : Type} (o : γ) : value (data α γ)
